

COMP4670 Assignment 1 Theory Answers

Jieli Zheng

u6579712

Exercise 1 Properties of Independent Variables

1

By definition of expectation of a continuous random variable:

$$\mathbf{E}_X = \int_{\Omega} X(\omega) dP(\omega), \text{ where } x, y, x + y \in \Omega$$

Therefore,

$$\begin{aligned} \mathbf{E}_{X,Y}[x + y] &= \iint (x + y) f(x, y) dx dy, \text{ f is the probability density function of } x, y \\ &= \iint x f(x, y) dx dy + \iint y f(x, y) dx dy \\ &= \mathbf{E}_X[x] + \mathbf{E}_Y[y] \quad \text{Q.E.D.} \end{aligned}$$

2

By definition of expectation of a continuous random variable:

$$\mathbf{E}_X = \int_{\Omega} X(\omega) dP(\omega), \text{ where } x, y, xy \in \Omega$$

Therefore,

$$\begin{aligned} \mathbf{E}_{X,Y}[xy] &= \iint xy f(x, y) dx dy, \text{ f is the probability density function of } x, y \\ &\text{Because X and Y are independent from each other, we have } f(x, y) = f(x)f(y) \end{aligned}$$

Then we have

$$\begin{aligned} \mathbf{E}_{X,Y}[xy] &= \iint xy f(x) f(y) dx dy \\ &= \int x f(x) dx \int y f(y) dy \\ &= \mathbf{E}_X \mathbf{E}_Y \quad \text{Q.E.D.} \end{aligned}$$

3

By definition of covariance:

$$cov[x, y] = \mathbf{E}_{X,Y}[x - \mathbf{E}_X[x])(y - \mathbf{E}_Y[y])]$$

Therefore,

$$cov[x, y] = \mathbf{E}[xy - y\mathbf{E}_X[x] - x\mathbf{E}_Y[y] + \mathbf{E}_X\mathbf{E}_Y]$$

From the proof mentioned in 1.1,1.2:

$$\mathbf{E}_{X,Y}[xy] = \mathbf{E}_X\mathbf{E}_Y \quad (1)$$

$$\mathbf{E}_{X,Y}[x + y] = \mathbf{E}_X[x] + \mathbf{E}_Y[y] \quad (2)$$

we have

$$\begin{aligned} cov[x, y] &= \mathbf{E}[xy] - \mathbf{E}[\mathbf{E}_X[x]y] - \mathbf{E}[\mathbf{E}_Y[y]x] + \mathbf{E}[\mathbf{E}_X\mathbf{E}_Y] \\ &= \mathbf{E}_{X,Y} - \mathbf{E}_X\mathbf{E}_Y - \mathbf{E}_Y\mathbf{E}_X + \mathbf{E}_{X,Y} \\ &= \mathbf{E}_{X,Y} - \mathbf{E}_X\mathbf{E}_Y \\ &= 0 \quad Q.E.D. \end{aligned}$$

Exercise 2 Beta Priors

1

$$B(a, b) = \int_0^1 x^{a-1}(1-x)^{b-1} dx, \text{ where } a, b \geq 1$$

Use Integration by substitution,

$$= \frac{1}{a} \int_0^1 (1-x)^{b-1} d(x^a)$$

Use Integration by parts,

$$\begin{aligned} &= (x^{a-1}(1-x)^{b-1}) \Big|_0^1 - \frac{1}{b} \int_0^1 x^{a-1} d(1-x)^b \\ &= 0 + \frac{1}{b} \int_0^1 x^{a-1} dx^b \\ &= \int_0^1 x^{a-1} x^{b-1} dx \\ &= \int_0^1 x^{a+b-2} dx \\ &= \frac{1}{a+b-1} x^{a+b-1} \Big|_0^1 \\ &= \frac{1}{a+b-1} (1-0) \\ &a+b-1 \geq 1, \text{ given } a, b \geq 1 \\ &\text{Therefore, } \frac{1}{a+b-1} \in (0, 1] \quad \text{Q.E.D.} \end{aligned}$$

2

First of all ,to prove $Beta(x|a, b)$ is a valid probability distribution, we need to prove:

- (1) $\forall x \in [0, 1], Beta(x|a, b) > 0$
- (2) $\int_0^1 Beta(x|a, b) = 1$

Proof of (1):

$$Beta(x|a, b) = \frac{1}{B(a, b)} x^{a-1} (1-x)^{b-1}$$

$$\text{Also from 2.1, } B(a, b) = \frac{1}{a+b-1}$$

$$\text{Therefore, } Beta(x|a, b) = (a+b-1)x^{a-1}(1-x)^{b-1}$$

Since $a, b \geq 1$

Then $a+b-1 \geq 1 \geq 0$

Because $x \in [0, 1]$

$$\forall m \in \mathcal{R} \quad x^m > 0$$

(except for 0, where 0^0 can be defined as 1 or remain undefined)

Hence $x^{a-1} > 0$, $(1-x)^{b-1} > 0$

Therefore, $Beta(x|a, b) = (a+b-1)x^{a-1}(1-x)^{b-1} \geq 0$ because 3 multipliers are all non-negative.

Proof of (2):

According to Exercise 2.1,

$$\begin{aligned} \int_0^1 Beta(x|a, b) &= \frac{1}{B(a, b)} \int_0^1 x^{a-1} (1-x)^{b-1} dx \\ &\text{because } \frac{1}{B(a, b)} \text{ is a constant according to 2.1} \\ &= \frac{1}{a+b-1} * (a+b-1) \\ &= 1 \end{aligned}$$

Therefore, the integral of PDF $Beta(x|a, b)$ is equal to 1.

Hence this PDF is a valid probability distribution.

Secondly, we need to prove $Beta(x|a, b)$ is well defined.

Because $B(a, b)$ (which is the denominator) is larger than 1, the only potential singular point for $Beta(x|a, b)$ is when $a = 1$, $x = 0$ or $b = 1$, $x = 1$ which makes a 0^0 .

However, usually 0^0 can be defined as 1.

Hence this PDF is a well defined probability distribution.

From the proofs above, we can say that $Beta(x|a, b)$ is a well defined and valid probability distribution.

3

By definition of Gamma function and Beta function by Gamma function,

$$\begin{aligned}\text{LEFT} &= \frac{\Gamma(a+1)\Gamma(b)}{\Gamma(a+b+1)} \\ &= \frac{a\Gamma(a)\Gamma(b)}{(a+b)\Gamma(a+b)} \\ &= \frac{a}{a+b} \frac{\Gamma(a)\Gamma(b)}{\Gamma(a+b)} \\ &= \text{RIGHT} \quad \text{Q.E.D.}\end{aligned}$$

Exercise 3 Coin Flips in Generality

1

Exercise 4 Noisy Coin Flips